feat: use absolute path names

lib/src/env.rs
@@ -1,13 +1,13 @@
-use crate::path::*;
 use crate::ty::*;
+
+use rustc_middle::ty::TyCtxt;
 use std::collections::HashMap;
 
 /// The environment used for the translation steps, holding various state
 /// information
-pub(crate) struct Env {
+pub(crate) struct Env<'a> {
     /// We use a counter for the disambiguation of several impls for the same
     /// type
     pub(crate) impl_counter: HashMap<CoqType, u64>,
-    /// The types that are currently in scope after a `use` statement
-    pub(crate) use_types: HashMap<String, Path>,
+    pub(crate) tcx: TyCtxt<'a>,
 }
