lib/src/path.rs
@@ -2,8 +2,8 @@ use crate::env::*;
 use crate::render::*;
 use rustc_hir::def::{CtorOf, DefKind, Res};
 use rustc_hir::{LangItem, QPath};
-use rustc_middle::ty::TyCtxt;
 use std::fmt;
+use std::vec;
 
 #[derive(Debug, Clone, PartialEq, Eq, Hash)]
 pub struct Path {
@@ -50,11 +50,19 @@ fn compile_path_without_env<Res>(path: &rustc_hir::Path<Res>) -> Path {
     }
 }
 
-pub(crate) fn compile_path<Res>(env: &Env, path: &rustc_hir::Path<Res>) -> Path {
-    if let [segment] = path.segments {
-        if let Some(path) = env.use_types.get(&segment.ident.name.to_string()) {
-            return path.clone();
-        }
+pub(crate) fn compile_path(env: &Env, path: &rustc_hir::Path) -> Path {
+    if let Some(def_if) = path.res.opt_def_id() {
+        let crate_name: String = env.tcx.crate_name(def_if.krate).to_string();
+        let path_items = env.tcx.def_path(def_if);
+        let mut segments = vec![crate_name];
+        segments.extend(
+            path_items
+                .data
+                .iter()
+                .filter_map(|item| item.data.get_opt_name())
+                .map(|name| to_valid_coq_name(name.to_string())),
+        );
+        return Path { segments };
     }
     compile_path_without_env(path)
 }
@@ -85,16 +93,17 @@ pub(crate) fn compile_qpath(env: &Env, qpath: &QPath) -> Path {
 }
 
 #[derive(Clone, Debug)]
-pub enum StructOrVariant {
+pub(crate) enum StructOrVariant {
     Struct,
     Variant,
 }
 
 impl StructOrVariant {
     /// Returns wether a qpath refers to a struct or a variant.
-    pub(crate) fn of_qpath(tcx: &TyCtxt, qpath: &QPath) -> StructOrVariant {
+    pub(crate) fn of_qpath(env: &Env, qpath: &QPath) -> StructOrVariant {
         let emit_warn_unsupported = || {
-            tcx.sess
+            env.tcx
+                .sess
                 .struct_span_warn(
                     qpath.span(),
                     "Cannot determine if this is a `struct` or an `enum`.",
@@ -143,18 +152,18 @@ impl StructOrVariant {
     }
 }
 
-pub fn to_valid_coq_name(str: String) -> String {
+pub(crate) fn to_valid_coq_name(str: String) -> String {
     let str = str::replace(&str, "$", "_");
     let str = str::replace(&str, "{{root}}", "Root");
     str::replace(&str, "::", ".")
 }
 
 impl Path {
-    pub fn to_doc(&self) -> Doc {
+    pub(crate) fn to_doc(&self) -> Doc {
         intersperse(self.segments.iter().map(text), [text(".")])
     }
 
-    pub fn to_name(&self) -> String {
+    pub(crate) fn to_name(&self) -> String {
         self.segments.join("_")
     }
 }
